going to adjust pair case

LeanLambdaLib/LambdaLib/paper_example_2.lean
@@ -27,28 +27,22 @@ abbrev U := <λ env. U>
 
 abbrev lambda := <λ t env a. t ({pair} env a)>
 abbrev app := <λ t1 t2 env. (t1 env) (t2 env)>
-
-abbrev weaken := <λ t env. t ({proj1} env)>
-abbrev subLast := <λ t toSub env. t ({pair} env (toSub env))>
 end S
 
 inductive Var : QTerm → QTerm → QTerm → Prop where
 | zero : ∀{ctx T},
-  Var <{S.cons} {ctx} {T}> <{S.weaken} {T}> S.zero
+  Var <{S.cons} {ctx} {T}> <λ env. {T} ({S.proj1} env)> S.zero
 | succ : ∀{ctx A T s}, Var ctx A s
-  → Var <{S.cons} {ctx} {T}> <{S.weaken} {A}> <{S.succ} {s}>
+  → Var <{S.cons} {ctx} {T}> <λ env. {A} ({S.proj1} env)> <{S.succ} {s}>
 
 -- context → level → type → term → prop
 inductive Typed : QTerm → QTerm → QTerm → Prop where
 | lambda : ∀{ctx A B s},
-  Typed <{S.cons} {ctx} {A}> B s
-  → Typed ctx <{S.pi} {A} {B}> <{S.lambda} {s}>
-| alambda : ∀{ctx A B s},
   Typed ctx S.U A
   → Typed <{S.cons} {ctx} {A}> B s
   → Typed ctx <{S.pi} {A} {B}> <{S.lambda} {s}>
 | app : ∀{ctx A B s1 s2}, Typed ctx <{S.pi} {A} {B}> s1 → Typed ctx A s2
-  → Typed ctx <{S.subLast} {B} {s2}> <{S.app} {s1} {s2}>
+  → Typed ctx <λ env. {B} ({S.pair} env ({s2} env))> <{S.app} {s1} {s2}>
 | var : ∀{ctx T t}, Var ctx T t → Typed ctx T t
 | U : ∀{ctx}, Typed ctx S.U S.U
 | Pi : ∀{ctx A B}, Typed ctx S.U A
@@ -57,37 +51,15 @@ inductive Typed : QTerm → QTerm → QTerm → Prop where
 
 def mycast {A B} (a : A) (h : A = B) : B := cast h a
 macro "mega_lambda_solve" : tactic => `(tactic|
-  repeat (any_goals (first | fail_if_no_progress lambda_solve | rfl | congr 1)))
+  repeat (any_goals (first | fail_if_no_progress lambda_solve | rfl | congr)))
 
 -- macro "{" t:term:10 "}" : term => `(mycast $t ?_)
 macro "{" t:term:10 "}" : term => `(mycast $t ?_)
 
+open Typed
+
 example : Typed S.nil S.U S.U := by
-  eapply {Typed.app {Typed.app (.alambda .U (.alambda (.var {Var.zero}) (.var .zero))) .U} .U}
+  eapply {app {app (lambda U (lambda (var {Var.zero}) (.var .zero))) .U} .U}
   --
-  -- TODO: why do these things crash while mega_lambda_solve doesn't?
-  iterate 7 rotate_left
-  --
-  congr 1
-  lambda_solve
-  --
-  rotate_left
-  --
-  congr 1 <;> normalize
-  -- TODO: i need to fix lambda_solve pair case so that this next line WOULDN'T simplify this!!!
-  -- lambda_solve -- this shouldn't do the pair case, since its not vars!
-  --
-  --
-  rotate_right
-  --
-  -- OK, here we are
-  --
-  congr 1
-  --
-  lambda_solve <;> rfl
-  --
-  normalize
-  --
-  --
-  -- mega_lambda_solve
+  mega_lambda_solve
   --
